\documentclass{jsarticle}
\usepackage{amsmath,amssymb,amsfonts}
\begin{document}
Calculates groebner basis of 
\begin{itemize}
\item $x^{3}+(-2)xy$
\item $x^{2}y+(-2)y^{2}+x$
\end{itemize}  . 


$S(x^{3}+(-2)xy, x^{2}y+(-2)y^{2}+x) = (-1)x^{2}$.  

Not enough.  Appends \begin{itemize}
\item $(-1)x^{2}$
\end{itemize}  . 


$S(x^{3}+(-2)xy, (-1)x^{2}) = (-2)xy$.  

$S(x^{2}y+(-2)y^{2}+x, (-1)x^{2}) = (-2)y^{2}+x$.  

Not enough.  Appends \begin{itemize}
\item $(-2)xy$
\end{itemize}  . 


$S(x^{3}+(-2)xy, (-2)xy) = 0$.  

$S(x^{2}y+(-2)y^{2}+x, (-2)xy) = (-2)y^{2}+x$.  

$S((-1)x^{2}, (-2)xy) = 0$.  

Not enough.  Appends \begin{itemize}
\item $(-2)y^{2}+x$
\end{itemize}  . 


$S(x^{3}+(-2)xy, (-2)y^{2}+x) = 0$.  

$S(x^{2}y+(-2)y^{2}+x, (-2)y^{2}+x) = 0$.  

$S((-1)x^{2}, (-2)y^{2}+x) = 0$.  

$S((-2)xy, (-2)y^{2}+x) = 0$.  

Enough for groebner basis.  Result is \begin{itemize}
\item $x^{3}+(-2)xy$
\item $x^{2}y+(-2)y^{2}+x$
\item $(-1)x^{2}$
\item $(-2)xy$
\item $(-2)y^{2}+x$
\end{itemize}  . 


\end{document}

