Calculates groebner basis of 
\begin{itemize}
\item $(-1)z^{4}+x$
\item $(-1)z^{5}+y$
\end{itemize}  .


$\overline{S((-1)z^{4}+x, (-1)z^{5}+y)} = (-1)xz+y$.

Not enough.  Appends \begin{itemize}
\item $(-1)xz+y$
\end{itemize}  .


$\overline{S((-1)z^{4}+x, (-1)xz+y)} = yz^{3}+(-1)x^{2}$.

$\overline{S((-1)z^{5}+y, (-1)xz+y)} = 0$.

Not enough.  Appends \begin{itemize}
\item $yz^{3}+(-1)x^{2}$
\end{itemize}  .


$\overline{S((-1)z^{4}+x, yz^{3}+(-1)x^{2})} = 0$.

$\overline{S((-1)z^{5}+y, yz^{3}+(-1)x^{2})} = 0$.

$\overline{S((-1)xz+y, yz^{3}+(-1)x^{2})} = (-1)y^{2}z^{2}+x^{3}$.

Not enough.  Appends \begin{itemize}
\item $(-1)y^{2}z^{2}+x^{3}$
\end{itemize}  .


$\overline{S((-1)z^{4}+x, (-1)y^{2}z^{2}+x^{3})} = 0$.

$\overline{S((-1)z^{5}+y, (-1)y^{2}z^{2}+x^{3})} = 0$.

$\overline{S((-1)xz+y, (-1)y^{2}z^{2}+x^{3})} = x^{4}+(-1)y^{3}z$.

$\overline{S(yz^{3}+(-1)x^{2}, (-1)y^{2}z^{2}+x^{3})} = 0$.

Not enough.  Appends \begin{itemize}
\item $x^{4}+(-1)y^{3}z$
\end{itemize}  .


$\overline{S((-1)z^{4}+x, x^{4}+(-1)y^{3}z)} = 0$.

$\overline{S((-1)z^{5}+y, x^{4}+(-1)y^{3}z)} = 0$.

$\overline{S((-1)xz+y, x^{4}+(-1)y^{3}z)} = 0$.

$\overline{S(yz^{3}+(-1)x^{2}, x^{4}+(-1)y^{3}z)} = 0$.

$\overline{S((-1)y^{2}z^{2}+x^{3}, x^{4}+(-1)y^{3}z)} = 0$.

Enough for groebner basis.  Result is \begin{itemize}
\item $(-1)z^{4}+x$
\item $(-1)z^{5}+y$
\item $(-1)xz+y$
\item $yz^{3}+(-1)x^{2}$
\item $(-1)y^{2}z^{2}+x^{3}$
\item $x^{4}+(-1)y^{3}z$
\end{itemize}  .
$\blacksquare{}$
Minimalizes groebner basis
\begin{itemize}
\item $(-1)z^{4}+x$
\item $(-1)z^{5}+y$
\item $(-1)xz+y$
\item $yz^{3}+(-1)x^{2}$
\item $(-1)y^{2}z^{2}+x^{3}$
\item $x^{4}+(-1)y^{3}z$
\end{itemize}  .


$(-1)z^{5}+y$ is removed by $(-1)z^{4}+x$.

Minimalized groebner basis is
\begin{itemize}
\item $z^{4}+(-1)x$
\item $xz+(-1)y$
\item $yz^{3}+(-1)x^{2}$
\item $y^{2}z^{2}+(-1)x^{3}$
\item $x^{4}+(-1)y^{3}z$
\end{itemize}  .
$\blacksquare{}$

Reduce groebner basis
\begin{itemize}
\item $z^{4}+(-1)x$
\item $xz+(-1)y$
\item $yz^{3}+(-1)x^{2}$
\item $y^{2}z^{2}+(-1)x^{3}$
\item $x^{4}+(-1)y^{3}z$
\end{itemize}  .


Reducing: $\overline{z^{4}+(-1)x} = z^{4}+(-1)x$.

Reducing: $\overline{xz+(-1)y} = xz+(-1)y$.

Reducing: $\overline{yz^{3}+(-1)x^{2}} = yz^{3}+(-1)x^{2}$.

Reducing: $\overline{y^{2}z^{2}+(-1)x^{3}} = y^{2}z^{2}+(-1)x^{3}$.

Reducing: $\overline{x^{4}+(-1)y^{3}z} = x^{4}+(-1)y^{3}z$.

Reduced groebner basis is
\begin{itemize}
\item $x^{4}+(-1)y^{3}z$
\item $y^{2}z^{2}+(-1)x^{3}$
\item $yz^{3}+(-1)x^{2}$
\item $xz+(-1)y$
\item $z^{4}+(-1)x$
\end{itemize}  .
$\blacksquare{}$
